update sim

dimsum/iris/sim.v
@@ -1,21 +1,14 @@
 From iris.bi Require Import bi fixpoint.
 From iris.proofmode Require Import base proofmode classes.
 From iris.base_logic.lib Require Export fancy_updates.
+From iris.base_logic.lib Require Export ghost_var.
 From iris.bi Require Export weakestpre.
-From dimsum.core Require Export module.
-From dimsum.core Require Import trefines.
+From dimsum.core Require Export module trefines.
 From dimsum.core.iris Require Export ord_later.
 Set Default Proof Using "Type".
 
-Class Sim (PROP : bi) (E1 E2 : Type) :=
-  sim : coPset → E1 → E2 → (E1 → E2 → PROP) → PROP.
-(* We assume only one instance is ever in scope, hence no mode *)
-
-(* FIXME what are good levels for et, es? *)
-Notation "et '⪯{' E '}' es {{ Φ } }" := (sim E et es Φ) (at level 70, Φ at level 200,
-  format "'[hv' et  '/' '⪯{' E '}'  '/' es  '/' {{  '[ ' Φ  ']' } } ']'") : bi_scope.
-
-Structure mod_lang Σ EV := ModLang {
+(** * mod_lang *)
+Structure mod_lang EV Σ := ModLang {
   mexpr : Type;
   mtrans : mod_trans EV;
   mexpr_rel : mtrans.(m_state) → mexpr → Prop;
@@ -28,125 +21,349 @@ Global Arguments mstate_interp {_ _} _ _.
 
 Definition mexprO {Σ EV} {Λ : mod_lang Σ EV} := leibnizO (mexpr Λ).
 
-Class dimsumPreG (Σ : gFunctors) := RefirisPreG {
+(** * dimsumGS *)
+Class dimsumPreG (Σ : gFunctors) (E_s : Type) := RefirisPreG {
   dimsum_pre_invG :> invGpreS Σ;
   dimsum_pre_ord_laterG :> ord_laterPreG Σ;
+  dimsum_pre_ghost_varG_s :> ghost_varG Σ E_s;
 }.
 
-Class dimsumGS (EV : Type) (Σ : gFunctors) (Λ_t Λ_s : mod_lang Σ EV) := DimsumGS {
+Class dimsumGS (EV : Type) (Σ : gFunctors) (Λ_t Λ_s : mod_lang EV Σ) := DimsumGS {
   dimsum_invGS :> invGS_gen HasNoLc Σ;
   dimsum_ord_laterGS :> ord_laterGS Σ;
+  dimsum_ghost_varG_s :> ghost_varG Σ (mexpr Λ_s);
+  dimsum_ghost_var_s_name : gname;
 }.
 Global Opaque dimsum_invGS.
 
+(** * [sim_expr_s] *)
+Definition sim_expr_s `{!dimsumGS EV Σ Λ_t Λ_s} (q : Qp) (e : mexpr Λ_s) : iProp Σ :=
+  ghost_var dimsum_ghost_var_s_name q e.
+
+Notation "'⤇{' q } e" := (sim_expr_s q e)
+  (at level 20, format "'⤇{' q }  e") : bi_scope.
+Notation "'⤇' e" := (sim_expr_s (1/2) e)
+  (at level 20, format "'⤇'  e") : bi_scope.
+Notation "'⤇?' e" := (if e is Some e' then sim_expr_s (1/2) e' else True)%I
+  (at level 20, format "'⤇?'  e") : bi_scope.
+
+Section sim_expr.
+  Context `{!dimsumGS EV Σ Λ_t Λ_s}.
+
+  Lemma sim_expr_s_agree e1 e2 :
+    ⤇ e1 -∗ ⤇ e2 -∗ ⌜e1 = e2⌝.
+  Proof. iIntros "??". by iDestruct (ghost_var_agree with "[$] [$]") as %->. Qed.
+
+  Lemma sim_expr_s_update e' e1 e2 :
+    ⤇ e1 -∗ ⤇ e2 ==∗ ⤇ e' ∗ ⤇ e'.
+  Proof. iApply ghost_var_update_halves. Qed.
+End sim_expr.
+
+(** * [sim_pre] *)
 Definition sim_pre `{!dimsumGS EV Σ Λ_t Λ_s}
-    (sim : leibnizO coPset -d> mexprO -d> mexprO -d> (mexprO -d> mexprO -d> iPropO Σ) -d> iPropO Σ) :
-    leibnizO coPset -d> mexprO -d> mexprO -d> (mexprO -d> mexprO -d> iPropO Σ) -d> iPropO Σ := λ E e_t e_s Φ,
-  (∀ σ_t σ_s, ⌜mexpr_rel Λ_t σ_t e_t⌝ -∗ ⌜mexpr_rel Λ_s σ_s e_s⌝ -∗
-    ord_later_ctx -∗ mstate_interp Λ_t σ_t -∗ mstate_interp Λ_s σ_s ={E}=∗
-      (mstate_interp Λ_t σ_t ∗ mstate_interp Λ_s σ_s ∗ Φ e_t e_s) ∨
-      ∀ κ Pσ_t, ⌜(mtrans Λ_t).(m_step) σ_t κ Pσ_t⌝ ={E,∅}=∗ ▷ₒ
+    (sim : leibnizO coPset -d> mexprO -d> (mexprO -d> iPropO Σ) -d> iPropO Σ) :
+    leibnizO coPset -d> mexprO -d> (mexprO -d> iPropO Σ) -d> iPropO Σ := λ E e_t Φ,
+  (∀ σ_t σ_s e_s, ⌜mexpr_rel Λ_t σ_t e_t⌝ -∗ ⌜mexpr_rel Λ_s σ_s e_s⌝ -∗ ord_later_ctx -∗
+              ⤇ e_s -∗ mstate_interp Λ_t σ_t -∗ mstate_interp Λ_s σ_s ={E}=∗
+      (⤇ e_s ∗ mstate_interp Λ_t σ_t ∗
+         mstate_interp Λ_s σ_s ∗ Φ e_t) ∨
+      (∀ κ Pσ_t, ⌜(mtrans Λ_t).(m_step) σ_t κ Pσ_t⌝ ={E,∅}=∗ ▷ₒ
         ∃ Pσ_s, ⌜σ_s ~{mtrans Λ_s, option_trace κ}~>ₜ Pσ_s⌝ ∗
-          ∀ σ_s', ⌜Pσ_s σ_s'⌝ ={∅, E}=∗
-            ∃ σ_t' e_t' e_s', ⌜Pσ_t σ_t'⌝ ∗ ⌜mexpr_rel Λ_t σ_t' e_t'⌝ ∗ ⌜mexpr_rel Λ_s σ_s' e_s'⌝ ∗
-              (mstate_interp Λ_t σ_t' ∗ mstate_interp Λ_s σ_s' ∗ sim E e_t' e_s' Φ))%I.
+         ∀ σ_s', ⌜Pσ_s σ_s'⌝ ={∅}=∗ ∃ σ_t' e_t' e_s', ⌜Pσ_t σ_t'⌝ ∗
+            ⌜mexpr_rel Λ_t σ_t' e_t'⌝ ∗ ⌜mexpr_rel Λ_s σ_s' e_s'⌝ ∗ ⤇ e_s' ∗
+            |={∅, E}=> mstate_interp Λ_t σ_t' ∗ mstate_interp Λ_s σ_s' ∗ sim E e_t' Φ)
+      ∨ |={E,∅}=> ∃ Pσ_s, ⌜σ_s ~{mtrans Λ_s, tnil}~>ₜ Pσ_s⌝ ∗
+             ∀ σ_s', ⌜Pσ_s σ_s'⌝ ={∅}=∗ ∃ e_s', ⌜mexpr_rel Λ_s σ_s' e_s'⌝ ∗ ⤇ e_s' ∗
+            |={∅, E}=> mstate_interp Λ_t σ_t ∗ mstate_interp Λ_s σ_s' ∗ sim E e_t Φ)%I.
 
 Global Instance sim_pre_ne `{!dimsumGS EV Λ_t Λ_s Σ} n:
-  Proper ((dist n ==> dist n ==> dist n ==> dist n ==> dist n) ==> dist n ==> dist n ==> dist n ==> dist n ==> dist n) sim_pre.
+  Proper ((dist n ==> dist n ==> dist n ==> dist n) ==> dist n ==> dist n ==> dist n ==> dist n) sim_pre.
 Proof.
-  move => ?? Hsim ?? -> ?? -> ?? -> ?? HΦ. rewrite /sim_pre.
+  move => ?? Hsim ?? -> ?? -> ?? HΦ. rewrite /sim_pre.
   repeat (f_equiv || eapply Hsim || eapply HΦ || reflexivity).
 Qed.
 
 Lemma sim_pre_mono `{!dimsumGS EV Λ_t Λ_s Σ} sim1 sim2:
-  ⊢ □ (∀ E e_t e_s Φ, sim1 E e_t e_s Φ -∗ sim2 E e_t e_s Φ )
-  → ∀ E e_t e_s Φ , sim_pre sim1 E e_t e_s Φ -∗ sim_pre sim2 E e_t e_s Φ.
+  ⊢ □ (∀ E e_t Φ, sim1 E e_t Φ -∗ sim2 E e_t Φ )
+  → ∀ E e_t Φ , sim_pre sim1 E e_t Φ -∗ sim_pre sim2 E e_t Φ.
 Proof.
-  iIntros "#Hinner" (E e_t e_s Φ) "Hsim".
-  iIntros (σ_t σ_s ??) "#? Hσ_t Hσ_s".
-  iMod ("Hsim" with "[//] [//] [//] Hσ_t Hσ_s") as "[Hsim|Hsim]"; [by iLeft|iRight]. iModIntro.
-  iIntros (κ P_tσ ?). iMod ("Hsim" with "[//]") as "Hsim". iModIntro. iMod "Hsim" as (??) "Hsim".
-  iExists _. iSplit; [done|].
-  iIntros (??). iMod ("Hsim" with "[//]") as (??????) "[? [??]]". iModIntro.
-  iSplit!; [done..|]. iFrame. by iApply "Hinner".
+  iIntros "#Hinner" (E e_t Φ) "Hsim".
+  iIntros (σ_t σ_s e_s ??) "#? ? Hσ_t Hσ_s".
+  iMod ("Hsim" with "[//] [//] [//] [$] Hσ_t Hσ_s") as "[Hsim|[Hsim|Hsim]]";
+    [by iLeft|iRight; iLeft| iRight; iRight].
+  - iModIntro. iIntros (κ Pσ_t ?). iMod ("Hsim" with "[//]") as "Hsim". iModIntro. iMod "Hsim" as (??) "Hsim".
+    iExists _. iSplit; [done|].
+    iIntros (??). iMod ("Hsim" with "[//]") as (??????) "[? Hsim]". iModIntro.
+    iSplit!; [done..|]. iFrame. iMod "Hsim" as "[? [??]]". iModIntro. iFrame. by iApply "Hinner".
+  - iModIntro. iMod "Hsim" as (??) "Hsim". iModIntro. iExists _. iSplit; [done|].
+    iIntros (??). iMod ("Hsim" with "[//]") as (??) "[? Hsim]". iModIntro.
+    iExists _. iSplit; [done|]. iFrame. iMod "Hsim" as "[? [??]]". iModIntro. iFrame. by iApply "Hinner".
 Qed.
 
 Local Instance sim_pre_monotone `{!dimsumGS EV Σ Λ_t Λ_s} :
-  BiMonoPred (λ sim : prodO (prodO (prodO (leibnizO coPset) mexprO) mexprO) (mexprO -d> mexprO -d> iPropO Σ) -d> iPropO Σ, uncurry4 (sim_pre (curry4 sim))).
+  BiMonoPred (λ sim : prodO (prodO (leibnizO coPset) mexprO) (mexprO -d> iPropO Σ) -d> iPropO Σ, uncurry3 (sim_pre (curry3 sim))).
 Proof.
   constructor.
-  - iIntros (Φ Ψ ??) "#Hinner". iIntros ([[[??]?]?]) "Hsim" => /=. iApply sim_pre_mono; [|done].
-    iIntros "!>" (????) "HΦ". by iApply ("Hinner" $! (_, _, _, _)).
-  - move => sim Hsim n [[[E1 e_t1] e_s1] Φ1] [[[E2 e_t2] e_s2] Φ2] /= [[/=[/=??]?]?].
-    apply sim_pre_ne; eauto. move => ???????????? /=. by apply: Hsim.
+  - iIntros (Φ Ψ ??) "#Hinner". iIntros ([[??]?]) "Hsim" => /=. iApply sim_pre_mono; [|done].
+    iIntros "!>" (???) "HΦ". by iApply ("Hinner" $! (_, _, _)).
+  - move => sim Hsim n [[E1 e_t1] Φ1] [[E2 e_t2] Φ2] /= [[/=??]?].
+    apply sim_pre_ne; eauto. move => ????????? /=. by apply: Hsim.
 Qed.
 
-Definition sim_def `{!dimsumGS EV Σ Λ_t Λ_s} : Sim (iPropI Σ) (mexpr Λ_t) (mexpr Λ_s) :=
-  curry4 (bi_least_fixpoint (λ sim : prodO (prodO (prodO (leibnizO coPset) mexprO) mexprO) (mexprO -d> mexprO -d> iPropO Σ) -d> iPropO Σ, uncurry4 (sim_pre (curry4 sim)))).
+Definition sim_def `{!dimsumGS EV Σ Λ_t Λ_s} : coPset → mexpr Λ_t → (mexpr Λ_t → iProp Σ) → iProp Σ :=
+  curry3 (bi_least_fixpoint (λ sim : prodO (prodO (leibnizO coPset) mexprO) (mexprO -d> iPropO Σ) -d> iPropO Σ, uncurry3 (sim_pre (curry3 sim)))).
 Definition sim_aux : seal (@sim_def). Proof. by eexists. Qed.
-Definition sim' := sim_aux.(unseal).
-Global Arguments sim' {EV Σ Λ_t Λ_s _}.
-Global Existing Instance sim'.
+Definition sim := sim_aux.(unseal).
+Global Arguments sim {EV Σ Λ_t Λ_s _}.
 Lemma sim_eq `{!dimsumGS EV Σ Λ_t Λ_s} : sim = @sim_def EV Σ Λ_t Λ_s _.
 Proof. rewrite -sim_aux.(seal_eq) //. Qed.
 
+Notation "'TGT' et @ E {{ Φ } }" := (sim E et Φ%I) (at level 70, Φ at level 200,
+  format "'[hv' 'TGT'  et  '/' @  E  {{  '[ ' Φ  ']' } } ']'") : bi_scope.
+
+(** * [sim_both] *)
+Definition sim_both `{!dimsumGS EV Σ Λ_t Λ_s} (E : coPset) (e_t : mexpr Λ_t) (e_s : mexpr Λ_s) (Φ : mexpr Λ_t → mexpr Λ_s → iProp Σ) : iProp Σ :=
+  ⤇ e_s -∗ TGT e_t @ E {{ λ e_t', ∃ e_s', ⤇ e_s' ∗ Φ e_t' e_s' }}.
+Notation "et '⪯{' E '}' es {{ Φ } }" := (sim_both E et es Φ%I) (at level 70, Φ at level 200,
+  format "'[hv' et  '/' '⪯{' E '}'  '/' es  '/' {{  '[ ' Φ  ']' } } ']'") : bi_scope.
+
+(** * [sim_src] *)
+Definition sim_src `{!dimsumGS EV Σ Λ_t Λ_s}
+  (E : coPset) (κ : option EV) (e_s : mexpr Λ_s) (Φ : mexpr Λ_s → iProp Σ) : iProp Σ :=
+  ∀ σ_s, ⌜mexpr_rel Λ_s σ_s e_s⌝ -∗ ord_later_ctx -∗ mstate_interp Λ_s σ_s ={E,∅}=∗
+    ∃ Pσ_s, ⌜σ_s ~{mtrans Λ_s, option_trace κ}~>ₜ Pσ_s⌝ ∗
+       ∀ σ_s', ⌜Pσ_s σ_s'⌝ ={∅}=∗ ∃ e_s', ⌜mexpr_rel Λ_s σ_s' e_s'⌝ ∗ |={∅, E}=> mstate_interp Λ_s σ_s' ∗ Φ e_s'.
+
+Notation "'SRC' e @ κ ; E {{ Φ } }" := (sim_src E κ e Φ%I) (at level 70, Φ at level 200,
+  format "'[hv' 'SRC'  e  '/' @  κ ;  E  {{  '[ ' Φ  ']' } } ']'") : bi_scope.
+
+Notation "'SRC' e @ E {{ Φ } }" := (sim_src E None e Φ%I) (at level 70, Φ at level 200,
+  format "'[hv' 'SRC'  e  '/' @  E  {{  '[ ' Φ  ']' } } ']'") : bi_scope.
+
+
 Section sim.
 Context `{!dimsumGS EV Σ Λ_t Λ_s}.
-Implicit Types s : stuckness.
 Implicit Types P : iProp Σ.
-Implicit Types Φ : mexpr Λ_t → mexpr Λ_s → iProp Σ.
 
-(* Weakest pre *)
-Lemma sim_unfold E e_t e_s Φ:
-  e_t ⪯{E} e_s {{ Φ }} ⊣⊢ sim_pre (sim (PROP:=iPropI Σ)) E e_t e_s Φ.
+(** * Lemmas about [sim] *)
+Lemma sim_unfold E e_t Φ:
+  TGT e_t @ E {{ Φ }} ⊣⊢ sim_pre sim E e_t Φ.
 Proof. rewrite sim_eq /sim_def /curry3. apply: least_fixpoint_unfold. Qed.
 
-Lemma sim_strong_ind (R: leibnizO coPset -d> mexprO -d> mexprO -d> (mexprO -d> mexprO -d> iPropO Σ) -d> iPropO Σ):
-  NonExpansive4 R →
-  ⊢ (□ ∀ E e_t e_s Φ, sim_pre (λ E e_t e_s Ψ, R E e_t e_s Ψ ∧ e_t ⪯{E} e_s {{ Ψ }}) E e_t e_s Φ -∗ R E e_t e_s Φ)
-    -∗ ∀ E e_t e_s Φ, e_t ⪯{E} e_s {{ Φ }} -∗ R E e_t e_s Φ.
+Lemma sim_strong_ind (R: leibnizO coPset -d> mexprO -d> (mexprO -d> iPropO Σ) -d> iPropO Σ):
+  NonExpansive3 R →
+  ⊢ (□ ∀ E e_t Φ, sim_pre (λ E e_t Ψ, R E e_t Ψ ∧ TGT e_t @ E {{ Ψ }}) E e_t Φ -∗ R E e_t Φ)
+    -∗ ∀ E e_t Φ, TGT e_t @ E {{ Φ }} -∗ R E e_t Φ.
 Proof.
-  iIntros (Hne) "#HPre". iIntros (E e_t e_s Φ) "Hsim".
-  rewrite sim_eq {2}/sim_def {1}/curry4.
-  iApply (least_fixpoint_ind _ (uncurry4 R) with "[] Hsim").
-  iIntros "!>" ([[[??]?]?]) "Hsim" => /=. by iApply "HPre".
+  iIntros (Hne) "#HPre". iIntros (E e_t Φ) "Hsim".
+  rewrite sim_eq {2}/sim_def {1}/curry3.
+  iApply (least_fixpoint_ind _ (uncurry3 R) with "[] Hsim").
+  iIntros "!>" ([[??]?]) "Hsim" => /=. by iApply "HPre".
 Qed.
 
-Lemma sim_ind (R: leibnizO coPset -d> mexprO -d> mexprO -d> (mexprO -d> mexprO -d> iPropO Σ) -d> iPropO Σ):
-  NonExpansive4 R →
-  ⊢ (□ ∀ E e_t e_s Φ, sim_pre R E e_t e_s Φ -∗ R E e_t e_s Φ)
-    -∗ ∀ E e_t e_s Φ, e_t ⪯{E} e_s {{ Φ }} -∗ R E e_t e_s Φ .
+Lemma sim_ind (R: leibnizO coPset -d> mexprO -d> (mexprO -d> iPropO Σ) -d> iPropO Σ):
+  NonExpansive3 R →
+  ⊢ (□ ∀ E e_t Φ, sim_pre R E e_t Φ -∗ R E e_t Φ)
+    -∗ ∀ E e_t Φ, TGT e_t @ E {{ Φ }} -∗ R E e_t Φ .
 Proof.
-  iIntros (Hne) "#HPre". iApply sim_strong_ind. iIntros "!>" (E e_t e_s Φ) "Hsim".
+  iIntros (Hne) "#HPre". iApply sim_strong_ind. iIntros "!>" (E e_t Φ) "Hsim".
   iApply "HPre". iApply (sim_pre_mono with "[] Hsim").
-  iIntros "!>" (????) "[? _]". by iFrame.
+  iIntros "!>" (???) "[? _]". by iFrame.
 Qed.
 
-Lemma sim_stop' E e_t e_s Φ:
-  (|={E}=> Φ e_t e_s) -∗ e_t ⪯{E} e_s {{ Φ }}.
-Proof. rewrite sim_unfold. iIntros "HΦ" (σ_t σ_s ??) "? Hσ_t Hσ_s". iLeft. iFrame. Qed.
-Lemma sim_stop E e_t e_s Φ:
+Lemma sim_wand e_t E Φ Ψ:
+  TGT e_t @ E {{ Φ }} -∗
+  (∀ e_t, Φ e_t -∗ Ψ e_t) -∗
+  TGT e_t @ E {{ Ψ }}.
+Proof.
+  iIntros "Hsim Hwand".
+  pose (F := (λ E e_t Ψ, ∀ Φ, (∀ e_t', Ψ e_t' -∗ Φ e_t') -∗ TGT e_t @ E {{ Φ }})%I).
+  iAssert (∀ Φ, TGT e_t @ E {{ Φ }} -∗ F E e_t Φ)%I as "Hgen"; last first.
+  { iApply ("Hgen" with "Hsim"). done. }
+  iIntros (?) "Hsim".
+  iApply (sim_ind with "[] Hsim"). { solve_proper. }
+  iIntros "!>" (?? ?) "Hsim". iIntros (?) "Hc".
+  rewrite sim_unfold. iIntros (?????) "#? ? Hσ_t Hσ_s".
+  iMod ("Hsim" with "[//] [//] [$] [$] Hσ_t Hσ_s") as "[[?[?[??]]]|[Hsim|Hsim]]".
+  - iModIntro. iLeft. iFrame. by iApply "Hc".
+  - iModIntro. iRight. iLeft. iIntros (???). iMod ("Hsim" with "[//]") as "Hsim". do 2 iModIntro.
+    iDestruct "Hsim" as (??) "Hsim".
+    iExists _. iSplit; [done|]. iIntros (??). iMod ("Hsim" with "[//]") as (??????) "[? Hsim]".
+    iModIntro. iSplit!; [done..|]. iFrame. iMod "Hsim" as "[$ [$ Hsim]]". iModIntro.
+    by iApply "Hsim".
+  - iModIntro. iRight. iRight. iMod ("Hsim") as (??) "Hsim". iModIntro.
+    iExists _. iSplit; [done|]. iIntros (??). iMod ("Hsim" with "[//]") as (??) "[? Hsim]".
+    iModIntro. iSplit!; [done..|]. iFrame. iMod "Hsim" as "[$ [$ Hsim]]". iModIntro.
+    by iApply "Hsim".
+Qed.
+
+Lemma sim_bind e_t E Φ:
+  TGT e_t @ E {{ λ e_t', TGT e_t' @ E {{ Φ }} }} -∗
+  TGT e_t @ E {{ Φ }}.
+Proof.
+  iIntros "Hsim".
+  pose (F := (λ E e_t Ψ, ∀ Φ, (∀ e_t', Ψ e_t' -∗ TGT e_t' @ E {{ Φ }}) -∗ TGT e_t @ E {{ Φ }})%I).
+  iAssert (∀ Φ, TGT e_t @ E {{ Φ }} -∗ F E e_t Φ)%I as "Hgen"; last first.
+  { iApply ("Hgen" with "Hsim"). iIntros (?) "?". done. }
+  iIntros (?) "Hsim".
+  iApply (sim_ind with "[] Hsim"). { solve_proper. }
+  iIntros "!>" (?? ?) "Hsim". iIntros (?) "Hc".
+  rewrite sim_unfold. iIntros (?????) "#? ? Hσ_t Hσ_s".
+  iMod ("Hsim" with "[//] [//] [$] [$] Hσ_t Hσ_s") as "[[?[?[??]]]|[Hsim|Hsim]]".
+  - iDestruct ("Hc" with "[$]") as "Hc". rewrite {1}sim_unfold.
+    iApply ("Hc" with "[//] [//] [$] [$] [$] [$]").
+  - iModIntro. iRight. iLeft. iIntros (???). iMod ("Hsim" with "[//]") as "Hsim". do 2 iModIntro.
+    iDestruct "Hsim" as (??) "Hsim".
+    iExists _. iSplit; [done|]. iIntros (??). iMod ("Hsim" with "[//]") as (??????) "[? Hsim]".
+    iModIntro. iSplit!; [done..|]. iFrame. iMod "Hsim" as "[$ [$ Hsim]]". iModIntro.
+    by iApply "Hsim".
+  - iModIntro. iRight. iRight. iMod ("Hsim") as (??) "Hsim". iModIntro.
+    iExists _. iSplit; [done|]. iIntros (??). iMod ("Hsim" with "[//]") as (??) "[? Hsim]".
+    iModIntro. iSplit!; [done..|]. iFrame. iMod "Hsim" as "[$ [$ Hsim]]". iModIntro.
+    by iApply "Hsim".
+Qed.
+
+Lemma sim_stop E e_t Φ:
+  Φ e_t -∗ TGT e_t @ E {{ Φ }}.
+Proof. rewrite sim_unfold. iIntros "HΦ" (σ_t σ_s e_s' ??) "? ? Hσ_t Hσ_s". iLeft. by iFrame. Qed.
+
+(** * Lemmas about [sim_both] *)
+Lemma sim_both_to_tgt E e_t e_s Φ:
+  (⤇ e_s -∗ TGT e_t @ E {{ λ e_t', ∃ e_s', ⤇ e_s' ∗ Φ e_t' e_s' }}) -∗ e_t ⪯{E} e_s {{ Φ }}.
+Proof. done. Qed.
+
+Lemma sim_tgt_to_both E e_t e_s Φ:
+  ⤇ e_s -∗
+  e_t ⪯{E} e_s {{ λ e_t' e_s', ⤇ e_s' -∗ Φ e_t' }} -∗
+  TGT e_t @ E {{ Φ }}.
+Proof.
+  iIntros "He Hsim".
+  iDestruct ("Hsim" with "He") as "Hsim".
+  iApply (sim_wand with "Hsim"). iIntros (?) "[%[? Hsim]]".
+  by iApply "Hsim".
+Qed.
+
+Lemma sim_both_stop E e_t e_s Φ:
   Φ e_t e_s -∗ e_t ⪯{E} e_s {{ Φ }}.
-Proof. iIntros "HΦ". iApply sim_stop'. by iFrame. Qed.
+Proof. iIntros "HΦ ?". iApply sim_stop. iExists _. iFrame. Qed.
+
+(** * Lemmas about [sim_src] *)
+Lemma sim_tgt_to_src E e_t e_s Φ:
+  ⤇ e_s -∗
+  SRC e_s @ E {{ λ e_s', ⤇ e_s' -∗ TGT e_t @ E {{ Φ }} }} -∗
+  TGT e_t @ E {{ Φ }}.
+Proof.
+  iIntros "He Hsim".
+  rewrite {2}sim_unfold. iIntros (?????) "#? ???". iModIntro.
+  iDestruct (sim_expr_s_agree with "[$] [$]") as %->.
+  iRight. iRight. iMod ("Hsim" with "[//] [$] [$]") as (??) "Hsim".
+  iModIntro. iExists _. iSplit; [done|]. iIntros (??).
+  iMod ("Hsim" with "[//]") as (??) "Hsim".
+  iMod (sim_expr_s_update with "[$] [$]") as "[? ?]". iModIntro.
+  iExists _. iSplit; [done|]. iFrame.
+  iMod "Hsim" as "[$ Hsim]". iModIntro. by iApply "Hsim".
+Qed.
+
+Lemma sim_src_stop E e_s Φ:
+  Φ e_s -∗ SRC e_s @ E {{ Φ }}.
+Proof.
+  iIntros "HΦ" (σ_s ?) "??".
+  iApply fupd_mask_intro; [set_solver|]. iIntros "He".
+  iExists (σ_s =.). iSplit; [iPureIntro; tend|]. iIntros (? <-) "!>".
+  iExists _. iSplit; [done|]. iMod "He". by iFrame.
+Qed.
+
+(* From dimsum Require Import axioms. *)
+(* Lemma thas_trace_post κs (m : mod_trans EV) σ1 Pσ2: *)
+(*   σ1 ~{ m, κs }~>ₜ Pσ2 → *)
+(*   ∃ Pσ2' σ,  *)
+(*   σ1 ~{ m, κs }~>ₜ (λ _, False) ∨ ∃ σ, Pσ2 σ. *)
+(* Proof. *)
+(*   elim; clear. *)
+(*   - naive_solver. *)
+(*   - move => σ1 Pσ2 Pσ3 κ κs κs' ? ? IH ?. *)
+(*     have [?|HF]:= AxClassic (∀ σ2 : m_state m, Pσ2 σ2 → σ2 ~{ m, κs' }~>ₜ (λ _ : m_state m, False)). *)
+(*     + left. by tstep. *)
+(*     + have [?|?]:= AxClassic (∃ σ2, Pσ2 σ2 ∧ ¬ σ2 ~{ m, κs' }~>ₜ (λ _ : m_state m, False)). *)
+(*       naive_solver. *)
+(*       exfalso. apply: HF => σ3?. *)
+(*       have [//|?]:= AxClassic (σ3 ~{ m, κs' }~>ₜ (λ _ : m_state m, False)). naive_solver. *)
+(*   - move => T f σ κs Pσ _ IH Hsub. *)
+(*     have [[x ?]|?]:= AxClassic (∃ x : T, ¬ σ ~{ m, f x }~>ₜ (λ _, False)). naive_solver. *)
+(*     left. eapply TTraceAll; [|done] => x. *)
+(*     have [|]:= AxClassic (σ ~{ m, f x }~>ₜ (λ _ : m_state m, False)); naive_solver. *)
+(* Qed. *)
 
 
+Lemma sim_src_bind E e_s Φ κ:
+  SRC e_s @ E {{ λ e_s', SRC e_s' @ κ; E {{ Φ }} }} -∗
+  SRC e_s @ κ; E {{ Φ }}.
+Proof.
+  iIntros "HΦ" (σ_s ?) "#??".
+  iMod ("HΦ" with "[//] [$] [$]") as (? Ht) "Hsim".
+  (* iExists (locked _). iSplitR. 2: { *)
+    (* iModIntro. iIntros (? HP). unlock in HP. apply HP. } *)
+  (* iModIntro. iPureIntro. apply: (thas_trace_trans tnil); [done|]. *)
+  (* move => ??. unlock. *)
+  iAssert (|={∅}=> ∃ Pσ_s0, ∀ σ_s', ⌜Pσ_s σ_s'⌝ -∗
+                             ⌜σ_s' ~{ mtrans Λ_s, option_trace κ }~>ₜ Pσ_s0⌝ ∗ (∀ σ_s', ⌜Pσ_s0 σ_s'⌝ ={∅}=∗
+         ∃ e_s', ⌜mexpr_rel Λ_s σ_s' e_s'⌝ ∗ (|={∅,E}=> mstate_interp Λ_s σ_s' ∗ Φ e_s')))%I
+    with "[-]" as "Hs"; last first.
+  { iMod "Hs" as (Pσ_s') "Hs". iModIntro. iExists Pσ_s'. iSplit. {
+      admit: "provable".
+    }
+    iIntros (??). admit: "provable by discarding the first part of Hs".
+  }
+  admit: "How to swap these quantifiers?".
+Abort.
+(*
+  move: (Ht) => /thas_trace_post[?|[??]].
+  { iModIntro. iExists (λ _, False). iSplit. { iPureIntro. by apply: (thas_trace_trans tnil). }
+    by iIntros (??). }
+  iMod ("Hsim" with "[//]") as (??) ">[? Hsim]".
+  iMod ("Hsim" with "[//] [$] [$]") as (??) "?". iModIntro.
+  iExists _. iSplit. { iPureIntro. apply: (thas_trace_trans tnil); [done|].
+
+ iModIntro.
+
+  iApply fupd_mask_intro; [set_solver|]. iIntros "He".
+  iExists (σ_s =.). iSplit; [iPureIntro; tend|]. iIntros (? <-) "!>".
+  iExists _. iSplit; [done|]. iMod "He". by iFrame.
+Qed.
+*)
+
+Lemma sim_src_steps E e_s Φ κ:
+  (∀ σ_s, ⌜mexpr_rel Λ_s σ_s e_s⌝ -∗ mstate_interp Λ_s σ_s ==∗
+    ∃ Pσ_s, ⌜σ_s ~{mtrans Λ_s, option_trace κ}~>ₜ Pσ_s⌝ ∗
+     ∀ σ_s', ⌜Pσ_s σ_s'⌝ ==∗ ∃ e_s',
+       ⌜mexpr_rel Λ_s σ_s' e_s'⌝ ∗ mstate_interp Λ_s σ_s' ∗ Φ e_s') -∗
+  SRC e_s @ κ; E {{ Φ }}.
+Proof.
+Abort.
+(*   iIntros "HΦ" (σ_s ?) "??". *)
+(*   iApply fupd_mask_intro; [set_solver|]. iIntros "He". *)
+(*   iExists (σ_s =.). iSplit; [iPureIntro; tend|]. iIntros (? <-) "!>". *)
+(*   iExists _. iSplit; [done|]. iMod "He". by iFrame. *)
+(* Qed. *)
+
+(*
 Lemma sim_step E e_t e_s Φ:
-  (∀ σ_t σ_s κ Pσ_t, ⌜mexpr_rel Λ_t σ_t e_t⌝ -∗ ⌜mexpr_rel Λ_s σ_s e_s⌝ -∗
-    ⌜(mtrans Λ_t).(m_step) σ_t κ Pσ_t⌝ -∗ mstate_interp Λ_t σ_t -∗ mstate_interp Λ_s σ_s ={E,∅}=∗ ▷ₒ
+  (∀ σ_t σ_s κ Pσ_t, ⌜(mtrans Λ_t).(m_step) σ_t κ Pσ_t⌝ -∗ ⤇ₜ e_t -∗ ⤇ₛ e_s -∗ σ⤇ₜ σ_t -∗ σ⤇ₛ σ_s ={E,∅}=∗ ▷ₒ
       ∃ Pσ_s, ⌜σ_s ~{mtrans Λ_s, option_trace κ}~>ₜ Pσ_s⌝ ∗
          ∀ σ_s', ⌜Pσ_s σ_s'⌝ ={∅, E}=∗
-           ∃ σ_t' e_t' e_s', ⌜Pσ_t σ_t'⌝ ∗ ⌜mexpr_rel Λ_t σ_t' e_t'⌝ ∗ ⌜mexpr_rel Λ_s σ_s' e_s'⌝ ∗
-              (mstate_interp Λ_t σ_t' ∗ mstate_interp Λ_s σ_s' ∗ e_t' ⪯{E} e_s' {{ Φ }})) -∗
+           ∃ σ_t' e_t' e_s', ⌜Pσ_t σ_t'⌝ ∗ ⤇ₜ e_t' ∗ ⤇ₛ e_s' ∗ σ⤇ₜ σ_t' ∗ σ⤇ₛ σ_s' ∗ e_t' ⪯{E} e_s' {{ Φ }}) -∗
   e_t ⪯{E} e_s {{ Φ }}.
 Proof.
   iIntros "Hsim".
-  rewrite sim_unfold. iIntros (????) "#? Hσ_t Hσ_s !>". iRight. iIntros (???).
-  iMod ("Hsim" with "[//] [//] [//] [$] [$]") as "Hsim". do 2 iModIntro.
+  rewrite sim_unfold. iIntros (??) "#? ?? Hσ_t Hσ_s !>". iRight. iIntros (???).
+  iMod ("Hsim" with "[//] [$] [$] [$] [$]") as "Hsim". do 2 iModIntro.
   iDestruct "Hsim" as (??) "Hsim". iExists _. iSplit; [done|].
-  iIntros (??). iMod ("Hsim" with "[//]") as (??????) "[? Hsim]".
+  iIntros (??). iMod ("Hsim" with "[//]") as (????) "[? Hsim]".
   iModIntro. iSplit!; [done..|]. iFrame.
 Qed.
+*)
 
+(*
 Lemma sim_bind E e_t e_s Φ:
   e_t ⪯{E} e_s {{ λ e_t' e_s', e_t' ⪯{E} e_s' {{ Φ }} }} -∗ e_t ⪯{E} e_s {{ Φ }}.
 Proof.
@@ -157,37 +374,48 @@ Proof.
   iIntros (?) "Hsim".
   iApply (sim_ind with "[] Hsim"). { solve_proper. }
   iIntros "!>" (????) "Hsim". iIntros (?) "Hc".
-  rewrite sim_unfold. iIntros (????) "#? Hσ_t Hσ_s".
-  iMod ("Hsim" with "[//] [//] [//] Hσ_t Hσ_s") as "[[? [??]]|Hsim]".
+  rewrite sim_unfold. iIntros (??) "#? ?? Hσ_t Hσ_s".
+  iMod ("Hsim" with "[//] [$] [$] Hσ_t Hσ_s") as "[[? [?[?[??]]]]|Hsim]".
   - iDestruct ("Hc" with "[$]") as "Hc". rewrite sim_unfold.
-    iApply ("Hc" with "[//] [//] [//] [$] [$]").
+    iApply ("Hc" with "[//] [$] [$] [$] [$]").
   - iModIntro. iRight. iIntros (???). iMod ("Hsim" with "[//]") as "Hsim". do 2 iModIntro.
     iDestruct "Hsim" as (??) "Hsim".
-    iExists _. iSplit; [done|]. iIntros (??). iMod ("Hsim" with "[//]") as (??????) "[? [? HF]]". iModIntro.
-    iSplit!; [done..|]. iFrame. by iApply "HF".
+    iExists _. iSplit; [done|]. iIntros (??). iMod ("Hsim" with "[//]") as (????) "[? [? [? [? HF]]]]".
+    iModIntro. iSplit!; [done..|]. iFrame. by iApply "HF".
 Qed.
+*)
 
-(* TODO *)
-(* Definition sim_src (E : coPset) (κ : option EV) (e_s : mexpr Λ_s) (Φ : mexpr Λ_s → iProp Σ) := *)
-(*   ∀ σ_t σ_s, ⌜mexpr_rel Λ_s σ_s e_s⌝ -∗ state_interp σ_t σ_s ={E,∅}=∗ *)
-(*     ∃ Pσ_s, ⌜σ_s ~{mtrans Λ_s, option_trace κ}~>ₜ Pσ_s⌝ ∗ *)
-(*        ∀ σ_s', ⌜Pσ_s σ_s'⌝ ={∅, E}=∗ *)
-(*             ∃ e_s', ⌜mexpr_rel Λ_s σ_s' e_s'⌝ ∗ *)
-(*               (state_interp σ_t σ_s' ∗ Φ e_s'). *)
+(*
+Lemma sim_bind_src E e_t e_s Φ:
+  sim_src E None e_s (λ e_t' e_s', e_t' ⪯{E} e_s' {{ Φ }}) -∗ e_t ⪯{E} e_s {{ Φ }}.
+Proof.
+  iIntros "Hsrc".
+  rewrite sim_unfold. iIntros (??) "#? ?? Hσ_t Hσ_s".
+  iModIntro. iRight.
+  iIntros (???).
+  iMod ("Hsrc" with "[$] [$] [$]") as (??) "Hsim". iModIntro.
+  iMod ("Hsim" with "[//] [//] [//] [$] [$] Hσ_t Hσ_s") as "[[? [?[?[??]]]]|Hsim]".
+  - iDestruct ("Hc" with "[$]") as "Hc". rewrite sim_unfold.
+    iApply ("Hc" with "[//] [//] [//] [$] [$] [$] [$]").
+  - iModIntro. iRight. iIntros (???). iMod ("Hsim" with "[//]") as "Hsim". do 2 iModIntro.
+    iDestruct "Hsim" as (??) "Hsim".
+    iExists _. iSplit; [done|]. iIntros (??). iMod ("Hsim" with "[//]") as (??????) "[? [? [? [? HF]]]]".
+    iModIntro. iSplit!; [done..|]. iFrame. by iApply "HF".
+Qed.
+*)
 
 End sim.
 
-Theorem sim_adequacy Σ EV `{!dimsumPreG Σ} m_t m_s :
-  (∀ `{Hinv : !invGS_gen HasNoLc Σ} `{Hord : !ord_laterGS Σ},
+Theorem sim_adequacy Σ EV m_t m_s expr_t expr_s `{!dimsumPreG Σ expr_s} `{!Inhabited (expr_s)} :
+  (∀ `{Hinv : !invGS_gen HasNoLc Σ} `{Hord : !ord_laterGS Σ} γ_s,
     ⊢ |={⊤}=>
-     ∃ (expr_t expr_s : Type),
      ∃ (expr_rel_t : (m_trans m_t).(m_state) → expr_t → Prop),
      ∃ (expr_rel_s : (m_trans m_s).(m_state) → expr_s → Prop),
      ∃ (stateI_t : (m_trans m_t).(m_state) → iProp Σ),
      ∃ (stateI_s : (m_trans m_s).(m_state) → iProp Σ),
-       let Λ_t := ModLang Σ EV expr_t (m_trans m_t) expr_rel_t stateI_t in
-       let Λ_s := ModLang Σ EV expr_s (m_trans m_s) expr_rel_s stateI_s in
-       let _ : dimsumGS EV Σ Λ_t Λ_s := DimsumGS _ _ _ _ _ _
+       let Λ_t := ModLang EV Σ expr_t (m_trans m_t) expr_rel_t stateI_t in
+       let Λ_s := ModLang EV Σ expr_s (m_trans m_s) expr_rel_s stateI_s in
+       let _ : dimsumGS EV Σ Λ_t Λ_s := DimsumGS _ _ _ _ _ _ _ γ_s
        in
        ∃ e_t e_s,
        ⌜mexpr_rel Λ_t m_t.(m_init) e_t⌝ ∗ ⌜mexpr_rel Λ_s m_s.(m_init) e_s⌝ ∗
@@ -198,25 +426,57 @@ Proof.
   intros Hsim. constructor => κs /thas_trace_n [n Htrace].
   apply (step_fupdN_soundness_no_lc _ 0 0) => ? /=. simpl in *. iIntros "_".
   iMod (ord_later_alloc n) as (?) "Ha". iDestruct (ord_later_ctx_alloc with "Ha") as "#?".
-  iMod Hsim as "(%expr_t & %expr_s & % & % & %stateI_t & %stateI_s & % & % & %He_t & %He_s & Hσ_t & Hσ_s & Hsim)".
+  iMod (ghost_var_alloc inhabitant) as (γ_s) "Hs".
+  iMod Hsim as "(% & % & %stateI_t & %stateI_s & % & % & %He_t & %He_s & Hσ_t & Hσ_s & Hsim)".
   clear Hsim.
-  set (σ_t := m_init m_t) in *. set (σ_s := m_init m_s) in *. clearbody σ_t σ_s.
-  iInduction Htrace as [????? Hκs|???????? Hstep ?? Hlt Hκs|????????? Hκs Hle] "IH" forall (σ_s e_t e_s He_t He_s).
-  - rewrite -Hκs. iApply fupd_mask_intro; [done|]. iIntros "HE". iPureIntro. by econstructor.
-  - rewrite -Hκs. setoid_rewrite sim_unfold at 2.
-    iMod ("Hsim" with "[//] [//] [//] Hσ_t Hσ_s") as "[[? [? Hsim]]|Hsim]". { by iMod "Hsim". }
+  set (Λ_t := ModLang EV Σ expr_t (m_trans m_t) expr_rel_t stateI_t).
+  set (Λ_s := ModLang EV Σ expr_s (m_trans m_s) expr_rel_s stateI_s).
+  set (X := DimsumGS _ _ _ _ _ _ _ γ_s : dimsumGS EV Σ Λ_t Λ_s).
+  iAssert (|==> ⤇ (e_s : mexpr Λ_s) ∗ ⤇ (e_s : mexpr Λ_s))%I with "[Hs]" as ">[He1 He2]".
+  { by iMod (ghost_var_update e_s with "Hs") as "[$ $]". }
+  pose (F := (λ E e_t Ψ,
+               ∀ n κs σ_s σ_t e_s,
+               ⌜σ_t ~{ m_trans m_t, κs, n }~>ₜ -⌝ -∗
+               ⌜expr_rel_t σ_t e_t⌝ -∗
+               ⌜expr_rel_s σ_s e_s⌝ -∗
+               ⌜E = ⊤⌝ -∗
+               ord_later_auth n -∗
+               ⤇ (e_s : mexpr Λ_s) -∗
+               stateI_t σ_t -∗
+               stateI_s σ_s -∗
+               (∀ e_t' : mexpr Λ_t, Ψ e_t' ={⊤,∅}=∗ False) -∗
+               |={⊤,∅}=> ⌜σ_s ~{ m_trans m_s, κs }~>ₜ -⌝)%I
+          : coPset → mexpr Λ_t → _ → iProp Σ ).
+  iAssert (∀ Φ, TGT (e_t : mexpr Λ_t) @ ⊤ {{ Φ }} -∗ F ⊤ e_t Φ)%I as "Hgen"; last first. {
+    iApply ("Hgen" with "[He1 Hsim] [//] [//] [//] [//] [$] [$] [$] [$]").
+    - by iApply "Hsim".
+    - iIntros (?) "[% [?$]]".
+  }
+  clear n κs Htrace e_s He_s He_t. iIntros (?) "Hsim".
+  iApply (sim_ind with "[] Hsim"). { solve_proper. }
+  iIntros "!>" (?? ?) "Hsim". iIntros (n κs σ_s σ_t e_s Htrace He_t He_s ->) "Ha He Hσ_t Hσ_s Hc".
+  iMod ("Hsim" with "[//] [//] [$] [$] Hσ_t Hσ_s") as "[[?[?[??]]]|[Hsim|Hsim]]".
+  - by iMod ("Hc" with "[$]").
+  - move: Htrace => /tnhas_trace_inv Htrace.
+    iApply (fupd_mono _ _ ⌜_⌝). { iPureIntro. by apply: thas_trace_under_tall. }
+    iIntros (?[[??]|[?[?[?[?[?[?[<- ?]]]]]]]]).
+    { iApply fupd_mask_intro; [done|]. iIntros "_". iPureIntro. tend. }
     iMod ("Hsim" with "[//]") as "Hsim" => /=.
     iMod (ord_later_elim with "Hsim Ha [-]"); [|done]. iIntros "Ha".
     iMod (ord_later_update with "Ha"); [shelve|].
     iModIntro. iExists _. iFrame. iSplit; [done|]. iIntros "Ha".
-    iDestruct 1 as (? Ht) "Hsim".
+    iDestruct 1 as (? Ht) "Hsim". iModIntro.
     iApply (fupd_mono _ _ ⌜_⌝). { iPureIntro. by apply thas_trace_trans. }
-    iModIntro. iIntros (??).
-    iMod ("Hsim" with "[//]") as (σ_t' ???? ?) "[Hσ_t [Hσ_s Hsim]]".
+    iIntros (??).
+    iMod ("Hsim" with "[//]") as (σ_t' ???? ?) "[? >[Hσ_t [Hσ_s Hsim]]]".
     iMod (ord_later_update with "Ha") as "Ha"; [by apply: o_le_choice_r|].
-    iApply ("IH" with "[//] [//] Ha Hσ_t Hσ_s Hsim").
-    Unshelve. { by apply o_lt_impl_le. } { done. }
-  - rewrite -Hκs. iApply (fupd_mono _ _ ⌜_⌝). { iPureIntro. apply thas_trace_all. }
-    iIntros (?). iMod (ord_later_update with "Ha") as "Ha". { etrans; [|done]. by apply: o_le_choice_r. }
-    iApply ("IH" with "[//] [//] Ha Hσ_t Hσ_s Hsim").
+    iApply ("Hsim" with "[//] [//] [//] [//] Ha [$] [$] [$] [$]").
+  - iMod "Hsim" as (??) "Hcont".
+    iApply (fupd_mono _ _ ⌜_⌝). { iPureIntro. by apply (thas_trace_trans tnil). }
+    iIntros (??). iMod ("Hcont" with "[//]") as (??) "[?>[?[? Hsim]]]".
+    iApply ("Hsim" with "[//] [//] [//] [//] [$] [$] [$] [$] [$]").
+  Unshelve.
+  + apply _.
+  + etrans; [|done]. apply o_le_S.
+  + done.
 Qed.
