dimsum/iris/language.v
@@ -1,43 +1,118 @@
 From iris.program_logic Require Export language.
-From iris.program_logic Require Import weakestpre.
+From iris.program_logic Require Import weakestpre lifting.
 From dimsum.core.iris Require Export sim.
+From dimsum.core Require Import axioms.
 Set Default Proof Using "Type".
 
 Definition nb_step EV (_ : unit) (_ : option EV) (_ : unit → Prop) : Prop := False.
 Definition nb_trans EV : mod_trans EV := ModTrans (nb_step EV).
-Canonical Structure nb_mod_lang EV : mod_lang EV := {|
+Canonical Structure nb_mod_lang EV Σ : mod_lang EV Σ := {|
   mexpr := unit;
   mtrans := nb_trans EV;
   mexpr_rel _ _ := True;
+  mstate_interp _ := True%I;
 |}.
 
 Inductive lang_step (Λ : language) :
   (expr Λ * state Λ) → option (observation Λ) → ((expr Λ * state Λ) → Prop) → Prop :=
 | LangStep e σ e' σ' efs κs :
   prim_step e σ κs e' σ' efs →
-  lang_step Λ (e, σ) (head κs) (λ σ'', σ'' = (e', σ')).
+  lang_step Λ (e, σ) (head κs) (λ σ'', σ'' = (e', σ'))
+| LangUbStep e σ :
+  ¬ reducible e σ →
+  lang_step Λ (e, σ) None (λ σ'', False).
 
 Definition lang_trans (Λ : language) : mod_trans (observation Λ) :=
   ModTrans (lang_step Λ).
 
-Canonical Structure lang_mod_lang (Λ : language) : mod_lang (observation Λ) := {|
+Canonical Structure lang_mod_lang {Σ} (Λ : language) (stateI : state Λ → iProp Σ) : mod_lang (observation Λ) Σ := {|
   mexpr := expr Λ;
   mtrans := lang_trans Λ;
   mexpr_rel σ e := e = σ.1;
+  mstate_interp σ := stateI σ.2;
 |}.
 
 Section wp.
   Context {Λ : language}.
   Context `{!irisGS_gen HasNoLc Λ Σ}.
 
-  Lemma sim_wp_adequacy e E Φ `{!ord_laterPreG Σ}:
-    (∀ γ_ord,
-      let _ : ord_laterGS Σ := OrdLaterGS _ _ γ_ord in
-      ∃ (stateI : (lang_trans Λ).(m_state) → (nb_trans _).(m_state) → iProp Σ),
-      (* TODO: Add a proof that the two state interpretations coincide. *)
-      let _ : dimsumGS _ (lang_mod_lang Λ) (nb_mod_lang _) Σ := DimsumGS _ _ _ _ _ _ stateI in
-     e ⪯{E} tt {{ λ e _, ∃ v, ⌜to_val e = Some v⌝ ∗ Φ v }}) -∗
-    WP e @ E {{ Φ }}.
+  Lemma sim_wp_adequacy e E `{!ord_laterPreG Σ}
+    `{!ghost_varG Σ unit}:
+    (∀ (e : expr Λ) σ κ e2 σ2 efs, prim_step e σ κ e2 σ2 efs → efs = []) →
+    (∀ σ ns κs nt, state_interp σ ns κs nt ⊣⊢ state_interp σ 0 [] 0) →
+    (∀ (Hord : ord_laterGS Σ) γ_s,
+      let Λ_t := lang_mod_lang Λ (λ σ, state_interp σ 0 [] 0) in
+      let _ : dimsumGS _ _ Λ_t (nb_mod_lang _ _) := DimsumGS _ _ _ _ _ _ _ γ_s in
+     (e : mexpr Λ_t) ⪯{E} tt {{ λ e _, ∃ v, ⌜to_val e = Some v⌝ }}) -∗
+    WP e @ E {{ _, True }}.
   Proof.
-  Abort.
+    iIntros (Hnofork Hstate) "Hsim".
+    iAssert (∃ n : nat, ▷^n False)%I as (n) "Hend".
+    { iLöb as "IH". iDestruct "IH" as (?) "IH". by iExists (S n). }
+    iMod (ord_later_alloc (nat_to_ord n)) as (?) "Hord".
+    iDestruct (ord_later_ctx_alloc with "[$]") as "#?".
+    iMod (ghost_var_alloc tt) as (γ_s) "Hs".
+    set (Λ_t := lang_mod_lang Λ (λ σ, state_interp σ 0 [] 0)).
+    set (X := DimsumGS _ _ _ _ _ _ _ γ_s : dimsumGS _ _ Λ_t (nb_mod_lang _ _)).
+    iAssert (|==> ⤇ tt ∗ ⤇ tt)%I with "[Hs]" as ">[He1 He2]".
+    { by iMod (ghost_var_update tt with "Hs") as "[$ $]". }
+    pose (F := (λ E e_t Ψ,
+               ∀ n,
+                 ▷^n False -∗
+                 ord_later_auth (nat_to_ord n) -∗
+                 ⤇ () -∗
+                 (∀ e_t' : mexpr Λ_t, Ψ e_t' -∗ ∃ v, ⌜to_val e_t' = Some v⌝) -∗
+                 WP e_t @ E {{ _, True }})%I
+                 : coPset → mexpr Λ_t → _ → iProp Σ ).
+  iAssert (∀ Φ, TGT e @ E {{ Φ }} -∗ F E e Φ)%I as "Hgen"; last first. {
+    iApply ("Hgen" with "[He1 Hsim] [$] [$] [$]").
+    - by iApply "Hsim".
+    - iIntros (?) "[% [?$]]".
+  }
+  iClear "Hend". clear n. iIntros (?) "Hsim".
+  iApply (sim_ind with "[] Hsim"). { solve_proper. }
+  iIntros "!>" (? e_t ?) "Hsim". iIntros (n) "Hend Hord He Hc".
+  destruct (to_val e_t) eqn:He.
+  { apply of_to_val in He. subst. by iApply wp_value'. }
+  rewrite wp_unfold /wp_pre. simplify_option_eq.
+  iIntros (σ ????) "Hσ".
+  iMod ("Hsim" $! (_, _) with "[//] [//] [//] [$] [Hσ] [//]") as "[[?[?[??]]]|[Hsim|Hsim]]".
+  { simpl. by rewrite -Hstate. }
+  { iDestruct ("Hc" with "[$]") as %[??]. simplify_eq. }
+  - destruct n; [done|] => /=.
+    have [Hred|Hnotred] := AxClassic (reducible e_t σ).
+    + iApply fupd_mask_intro; [set_solver|]. iIntros "He". iSplit; [done|].
+      iIntros (????) "_ !> !> !>". iApply step_fupdN_intro; [done|]. iModIntro. iMod "He".
+      iMod ("Hsim" with "[%]") as "Hsim". { by econstructor. }
+      iMod (ord_later_elim with "Hsim Hord [-]"); [|done]. iIntros "Hord /=".
+      iMod (ord_later_update with "Hord"); [by apply o_le_S|].
+      iModIntro. iExists _. iFrame. iSplit; [done|]. iIntros "Hod".
+      iDestruct 1 as (? Ht) "Hsim". iModIntro.
+      iMod ("Hsim" $! tt with "[%]") as (?????) "[?[? >[Hσ [? Hsim]]]]". {
+          destruct κ.
+          - apply thas_trace_nil_inv in Ht. by inv Ht.
+          - apply thas_trace_cons_inv in Ht.
+            apply thas_trace_nil_inv in Ht. inv Ht => //. destruct!.
+            inv_all @m_step.
+        }
+        exploit Hnofork; [done|] => ?. simplify_eq/=. destruct_all unit. iModIntro.
+        iSplitL "Hσ". { by iApply Hstate. }
+        iSplit; [|done]. iApply ("Hsim" with "[$] [$] [$] [$]").
+      + iMod ("Hsim" with "[%]") as "Hsim". { by constructor. }
+        iMod (ord_later_elim with "Hsim Hord [-]"); [|done]. iIntros "Hord/=".
+        iMod (ord_later_update with "Hord"); [by apply o_le_S|].
+        iModIntro. iExists _. iFrame. iSplit; [done|]. iIntros "Hod".
+        iDestruct 1 as (? Ht) "Hsim". iModIntro.
+        iMod ("Hsim" $! tt with "[%]") as (??????) "[? ?]".
+        { apply thas_trace_nil_inv in Ht. by inv Ht. }
+        done.
+  - iMod "Hsim" as (? Ht) "Hsim".
+    iMod ("Hsim" $! tt with "[%]") as (??) "[? >[?[? Hsim]]]".
+    { apply thas_trace_nil_inv in Ht. by inv Ht. } simplify_eq/=. destruct_all unit.
+    iDestruct ("Hsim" with "[$] [$] [$] [$]") as "Hsim".
+    rewrite wp_unfold /wp_pre. simplify_option_eq.
+    iMod ("Hsim" with "[-]") as "Hsim".
+    { by rewrite -Hstate. }
+    done.
+  Qed.
 End wp.
